FOTheory.v
@@ -1,151 +1,195 @@
-Require Import Arith.
-Require Import List.
+Require Export Arith.
+Require Export Omega.
+Require Export List.
 
 Inductive foterm :=
-  | Val : nat -> foterm
-  | Cst_0 : foterm
-  | Cst_S : foterm -> foterm
-  | Df_Add : foterm -> foterm -> foterm.
+| Val : nat -> foterm
+| Cst_0 : foterm
+| Cst_1 : foterm
+| Df_Add : foterm -> foterm -> foterm.
 
-Fixpoint free_var_fotrm t : list nat:=
- match t with
- | Val n => n::nil
- | Cst_0 => nil
- | Cst_S N => free_var_fotrm N
- | Df_Add M N => (free_var_fotrm M) ++ (free_var_fotrm N)
- end.
-
-Inductive cst_clsd_trm : foterm -> Prop :=
-  | cct0 : cst_clsd_trm Cst_0
-  | cctS : forall y, cst_clsd_trm y -> cst_clsd_trm (Cst_S y).
-
-Parameter eq_fotrm : foterm -> foterm -> Prop.
-
-Axiom non_triviality : exists x y, 
-  cst_clsd_trm x /\ cst_clsd_trm y /\ ~ eq_fotrm x y.
-
-Axiom freeness : forall x y, 
-  cst_clsd_trm x -> 
-  cst_clsd_trm y -> 
-  eq_fotrm x y ->
-  x = y.
-
-Axiom completeness : forall x, free_var_fotrm x = nil ->
-  exists y, cst_clsd_trm y /\ eq_fotrm x y.
+Fixpoint free_var_fotrm t k : list nat :=
+  match t with
+    | Val n => 
+      match le_gt_dec k n with
+        | left _ => n::nil
+        | right _ => nil
+      end
+    | Cst_0 => nil
+    | Cst_1 => nil
+    | Df_Add M N => (free_var_fotrm M k) ++ (free_var_fotrm N k)
+  end.
 
 Fixpoint lift_trm_rec t n k:=
   match t with
-  | Val i => 
-    match le_gt_dec k i with
-    | left _ => Val (i+n)
-    | right _ => Val i
-    end
-  | Cst_0 => Cst_0
-  | Cst_S u => Cst_S (lift_trm_rec u n k)
-  | Df_Add u v => Df_Add (lift_trm_rec u n k) (lift_trm_rec v n k)
+    | Val i => 
+      match le_gt_dec k i with
+        | left _ => Val (i+n)
+        | right _ => Val i
+      end
+    | Cst_0 => Cst_0
+    | Cst_1 => Cst_1
+    | Df_Add u v => Df_Add (lift_trm_rec u n k) (lift_trm_rec v n k)
   end.
 
 Definition lift_trm t n := lift_trm_rec t n 0.
 
-Definition Cst_1 := Cst_S Cst_0.
+Fixpoint subst_trm_rec M N n:= 
+  match M with
+    | Val i =>
+      match lt_eq_lt_dec n i with
+        | inleft (left _) => Val (pred i)
+        | inleft (right _) => lift_trm N n
+        | inright _ => Val i
+      end
+    | Cst_0 => Cst_0
+    | Cst_1 => Cst_1
+    | Df_Add M1 M2 => Df_Add (subst_trm_rec M1 N n) (subst_trm_rec M2 N n)
+  end.
 
-Section presberger.
+Definition subst_trm M N := subst_trm_rec M N 0.
 
-  Parameter eq_discr : ~ eq_fotrm Cst_0 (Df_Add Cst_1 Cst_0).
+Lemma subst_bound_trm : forall t m, 
+  subst_trm_rec (lift_trm_rec t 1 (S m)) (Val 0) m = t.
+induction t; intros; trivial.
+ unfold lift_trm_rec. destruct (Compare_dec.le_gt_dec (S m) n).
+  simpl. destruct (Compare_dec.lt_eq_lt_dec m (n + 1)).
+   destruct s. 
+    rewrite Plus.plus_comm; simpl; trivial.
 
-  Parameter eq_inj : forall x y, eq_fotrm (Df_Add x Cst_1) (Df_Add y Cst_1).
+    rewrite e in l. apply Le.le_Sn_le in l. 
+    rewrite Plus.plus_comm in l. apply Le.le_Sn_n in l. contradiction.
 
-  Parameter eq_add0 : forall x, eq_fotrm x (Df_Add x Cst_0).
+    assert (m < n); trivial.
+    assert (n < n + 1) by omega.
+    generalize (Lt.lt_trans _ _ _ H0 l0); intros.
+    generalize (Lt.lt_trans _ _ _ H1 H); intros.
+    apply Lt.lt_irrefl in H2; contradiction.
 
-  Parameter add_assoc : forall x y, 
-    eq_fotrm (Df_Add (Df_Add x y) Cst_1) (Df_Add x (Df_Add y Cst_1)).
+  simpl. destruct (Compare_dec.lt_eq_lt_dec m n); trivial.
+   destruct s.
+    assert (S m <= n) by omega.
+    assert (n < S m) by omega.
+    generalize (Lt.le_lt_trans _ _ _ H H0); intros.
+    apply Lt.lt_irrefl in H1; contradiction.
 
-  Parameter ind_ax : forall P y, P Cst_0 ->
-    (forall x, P x -> P (Df_Add x Cst_1)) -> P y.
+    subst m. unfold lift_trm; simpl; trivial.
 
-End presberger.
+ simpl. rewrite IHt1, IHt2; trivial.
+Qed.
 
 Inductive foformula :=
-  | atom : (list foterm -> Prop) -> list foterm -> foformula
-  | TF   : foformula
-  | BF   : foformula
-  | neg : foformula -> foformula
-  | conj : foformula -> foformula -> foformula
-  | disj : foformula -> foformula -> foformula
-  | implf : foformula -> foformula -> foformula
-  | fall : foformula -> foformula
-  | exst : foformula -> foformula.
+| eq_fotrm : foterm -> foterm -> foformula
+| TF   : foformula
+| BF   : foformula
+| neg : foformula -> foformula
+| conj : foformula -> foformula -> foformula
+| disj : foformula -> foformula -> foformula
+| implf : foformula -> foformula -> foformula
+| fall : foformula -> foformula
+| exst : foformula -> foformula.
 
 Fixpoint lift_fml_rec f n k:=
   match f with
-  | atom P l => atom P (map (fun x => lift_trm_rec x n k) l)
-  | TF => TF
-  | BF => BF
-  | neg f' => neg (lift_fml_rec f' n k)
-  | conj A B => conj (lift_fml_rec A n k) (lift_fml_rec B n k)
-  | disj A B => disj (lift_fml_rec A n k) (lift_fml_rec B n k)
-  | implf A B => implf (lift_fml_rec A n k) (lift_fml_rec B n k)
-  | fall A => fall (lift_fml_rec A n (S k))
-  | exst A => exst (lift_fml_rec A n (S k))
+    | eq_fotrm x y => eq_fotrm (lift_trm_rec x n k) (lift_trm_rec y n k)
+    | TF => TF
+    | BF => BF
+    | neg f' => neg (lift_fml_rec f' n k)
+    | conj A B => conj (lift_fml_rec A n k) (lift_fml_rec B n k)
+    | disj A B => disj (lift_fml_rec A n k) (lift_fml_rec B n k)
+    | implf A B => implf (lift_fml_rec A n k) (lift_fml_rec B n k)
+    | fall A => fall (lift_fml_rec A n (S k))
+    | exst A => exst (lift_fml_rec A n (S k))
   end.
 
 Definition lift_fml t n := lift_fml_rec t n 0.
 
-Fixpoint subst_trm M N n:= 
-  match M with
-  | Val i =>
-    match lt_eq_lt_dec n i with
-    | inleft (left _) => Val (pred i)
-    | inleft (right _) => lift_trm N n
-    | inright _ => Val i
-    end
-  | Cst_0 => Cst_0
-  | Cst_S M' => Cst_S (subst_trm M' N n)
-  | Df_Add M1 M2 => Df_Add (subst_trm M1 N n) (subst_trm M2 N n)
-  end.
-
 Fixpoint subst_fml f N n :=
   match f with
-  | atom P l => atom P (map (fun M => subst_trm M N n) l)
-  | TF => TF
-  | BF => BF
-  | neg f => neg (subst_fml f N n)
-  | conj f1 f2 => conj (subst_fml f1 N n) (subst_fml f2 N n)
-  | disj f1 f2 => disj (subst_fml f1 N n) (subst_fml f2 N n)
-  | implf f1 f2 => implf (subst_fml f1 N n) (subst_fml f2 N n)
-  | fall f => fall (subst_fml f N (S n))
-  | exst f => exst (subst_fml f N (S n))
+    | eq_fotrm x y => eq_fotrm (subst_trm_rec x N n) (subst_trm_rec y N n)
+    | TF => TF
+    | BF => BF
+    | neg f => neg (subst_fml f N n)
+    | conj f1 f2 => conj (subst_fml f1 N n) (subst_fml f2 N n)
+    | disj f1 f2 => disj (subst_fml f1 N n) (subst_fml f2 N n)
+    | implf f1 f2 => implf (subst_fml f1 N n) (subst_fml f2 N n)
+    | fall f => fall (subst_fml f N (S n))
+    | exst f => exst (subst_fml f N (S n))
   end.
 
 Definition subst_fml0 f N := subst_fml f N 0.
 
-Definition hyp_ok (hyp:list (option foformula)) t := 
- forall n, In n (free_var_fotrm t) -> nth_error hyp n = Some None.
-
-Definition predicate_stable P := forall l n k N, 
-  (P l <-> P (map (fun x => lift_trm_rec x n k) l)) /\
-  (P l <-> P (map (fun M : foterm => subst_trm M N k) l)).
+Lemma subst_bound_fml : forall P m,
+  P = subst_fml (lift_fml_rec P 1 (S m)) (Val 0) m.
+induction P; simpl; intros; trivial.
+ do 2 rewrite subst_bound_trm; trivial.
  
+ rewrite <- IHP; trivial.
+
+ rewrite <- IHP1, <-IHP2; trivial.
+
+ rewrite <- IHP1, <-IHP2; trivial.
+
+ rewrite <- IHP1, <-IHP2; trivial.
+
+ rewrite <- IHP with (m:= S m); trivial.
+
+ rewrite <- IHP with (m:= S m); trivial.
+Qed.
+
+Definition P_ax f :=
+  f = (fall (neg (eq_fotrm Cst_0 (Df_Add (Val 0) Cst_1))))      \/
+  f = (fall (fall (implf (eq_fotrm (Df_Add (Val 0) Cst_1) 
+    (Df_Add (Val 1) Cst_1)) (eq_fotrm (Val 0) (Val 1)))))       \/
+  f = (fall (eq_fotrm (Val 0) (Df_Add (Val 0) Cst_0)))          \/
+  f = (fall(fall (eq_fotrm (Df_Add (Df_Add (Val 0) (Val 1)) Cst_1) 
+                   (Df_Add (Val 0) (Df_Add (Val 1) (Cst_1)))))) \/
+  exists g, f = (implf (subst_fml0 g Cst_0) 
+    (implf (fall (implf g 
+      (subst_fml0 (lift_fml_rec g 1 1) (Df_Add (Val 0) Cst_1)))) 
+    (fall g))).
+
+
+Definition hyp_ok (hyp:list (option foformula)) t := 
+  forall n, In n (free_var_fotrm t 0) -> nth_error hyp n = Some None.
+
 Inductive deriv : list (option foformula) -> foformula -> Prop :=
-  | weak : forall f hyp, deriv ((Some f)::hyp) (lift_fml f 1)
-  | atom_intro : forall (P : list foterm -> Prop) l hyp, 
-      predicate_stable P -> P l -> deriv hyp (atom P l)
-  | neg_intro : forall hyp f, deriv hyp (implf f BF) -> deriv hyp (neg f)
-  | conj_intro : forall hyp f1 f2 , 
-      deriv hyp f1 -> deriv hyp f2 -> deriv hyp (conj f1 f2)
-  | disj_intro1 : forall hyp f1 f2, 
-      deriv hyp f1 -> deriv hyp (disj f1 f2)
-  | disj_intro2 : forall hyp f1 f2, 
-      deriv hyp f2 -> deriv hyp (disj f1 f2)
-  | impl_intro : forall hyp f1 f2,
-      deriv ((Some f1)::hyp) (lift_fml f2 1) -> deriv hyp (implf f1 f2)
-  | fall_intro : forall hyp f,
-      deriv (None::hyp) f -> deriv hyp (fall f)
-  | exst_intro : forall hyp f N, hyp_ok hyp N -> 
-      deriv hyp (subst_fml0 f N) -> deriv hyp (exst f). 
+| weak : forall f hyp, deriv ((Some f)::hyp) (lift_fml f 1)
+| ax_intro : forall f hyp, P_ax f -> deriv hyp f
+| true_intro : forall hyp, deriv hyp TF
+| false_elim : forall hyp f, deriv hyp BF -> deriv hyp f
+| neg_intro : forall hyp f, deriv hyp (implf f BF) -> deriv hyp (neg f)
+| neg_elim : forall hyp f, deriv hyp (neg f) -> deriv hyp (implf f BF)
+| conj_intro : forall hyp f1 f2 , 
+  deriv hyp f1 -> deriv hyp f2 -> deriv hyp (conj f1 f2)
+| conj_elim1 : forall hyp f1 f2,
+  deriv hyp (conj f1 f2) -> deriv hyp f1
+| conj_elim2 : forall hyp f1 f2,
+  deriv hyp (conj f1 f2) -> deriv hyp f2
+| disj_intro1 : forall hyp f1 f2, 
+  deriv hyp f1 -> deriv hyp (disj f1 f2)
+| disj_intro2 : forall hyp f1 f2, 
+  deriv hyp f2 -> deriv hyp (disj f1 f2)
+| disj_elim : forall hyp f1 f2 f3,
+  deriv hyp (disj f1 f2) -> deriv (Some f1::hyp) (lift_fml f3 1) -> 
+  deriv (Some f2::hyp) (lift_fml f3 1) -> deriv hyp f3
+| impl_intro : forall hyp f1 f2,
+  deriv ((Some f1)::hyp) (lift_fml f2 1) -> deriv hyp (implf f1 f2)
+| impl_elim : forall hyp f1 f2,
+  deriv hyp (implf f1 f2) -> deriv hyp f1 -> deriv hyp f2
+| fall_intro : forall hyp f,
+  deriv (None::hyp) f -> deriv hyp (fall f)
+| fall_elim : forall hyp f u, hyp_ok hyp u ->
+  deriv hyp (fall f) -> deriv hyp (subst_fml0 f u)
+| exst_intro : forall hyp f N, hyp_ok hyp N -> 
+  deriv hyp (subst_fml0 f N) -> deriv hyp (exst f)
+| exst_elim : forall hyp f f1, deriv hyp (exst f) -> 
+  deriv (Some f::None::hyp) (lift_fml f1 2) -> deriv hyp f1.
 
 
 
 
 
 
+
+ 
